interface for LowParse.Spec.List

src/lowparse/LowParse.Spec.List.fst
@@ -8,133 +8,12 @@ module Classical = FStar.Classical
 
 (* Parse a list, until there is nothing left to read. This parser will mostly fail EXCEPT if the whole size is known and the slice has been suitably truncated beforehand, or if the elements of the list all have a known constant size. *)
 
-val parse_list_aux
-  (#k: parser_kind)
-  (#t: Type0)
-  (p: parser k t)
-  (b: bytes)
-: GTot (option (list t * (consumed_length b)))
-  (decreases (Seq.length b))
-
-let rec parse_list_aux #k #t p b =
-  if Seq.length b = 0
-  then 
-    Some ([], (0 <: consumed_length b))
-  else
-    match parse p b with
-    | None -> None
-    | Some (v, n) ->
-      if n = 0
-      then None (* elements cannot be empty *)
-      else
-        match parse_list_aux p (Seq.slice b n (Seq.length b)) with
-	| Some (l, n') -> Some (v :: l, (n + n' <: consumed_length b))
-	| _ -> None
-
-val parse_list_bare
-  (#k: parser_kind)
-  (#t: Type0)
-  (p: parser k t)
-: Tot (bare_parser (list t))
-
-let parse_list_bare #k #t p = (fun b -> parse_list_aux #k #t p b) <: bare_parser (list t)
-
-let rec parse_list_bare_consumed
-  (#k: parser_kind)
-  (#t: Type0)
-  (p: parser k t)
-  (b: bytes)
-: Lemma
-  (requires (Some? (parse_list_bare p b)))
-  (ensures (
-    let pb = parse_list_bare p b in (
-    Some? pb /\ (
-    let (Some (_, consumed)) = pb in
-    consumed == Seq.length b
-  ))))
-  (decreases (Seq.length b))
-= if Seq.length b = 0
-  then ()
-  else
-    let (Some (_, consumed1)) = p b in
-    let b' = Seq.slice b consumed1 (Seq.length b) in
-    parse_list_bare_consumed p b'
-
-let parse_list_bare_consumes_all
-  (#k: parser_kind)
-  (#t: Type0)
-  (p: parser k t)
-: Lemma
-  (consumes_all (parse_list_bare p))
-= Classical.forall_intro (Classical.move_requires (parse_list_bare_consumed p))
-
-#set-options "--z3rlimit 16"
-
-let parse_list_bare_injective
-  (#k: parser_kind)
-  (#t: Type0)
-  (p: parser k t)
-: Lemma
-  (ensures (injective (parse_list_bare p)))
-= parser_kind_prop_equiv k p;
-  let f () : Lemma
-    (injective p)
-  = ()
-  in
-  let rec aux
-    (b1: bytes)
-    (b2: bytes)
-  : Lemma
-    (requires (injective_precond (parse_list_bare p) b1 b2))
-    (ensures (injective_postcond (parse_list_bare p) b1 b2))
-    (decreases (Seq.length b1 + Seq.length b2))
-  = if Seq.length b1 = 0
-    then begin
-      () // assert (Seq.equal b1 b2)
-    end else begin
-      assert (injective_precond p b1 b2);
-      f ();
-      assert (injective_postcond p b1 b2);
-      let (Some (_, len1)) = parse p b1 in
-      let (Some (_, len2)) = parse p b2 in
-      assert ((len1 <: nat) == (len2 <: nat));
-      let b1' : bytes = Seq.slice b1 len1 (Seq.length b1) in
-      let b2' : bytes = Seq.slice b2 len2 (Seq.length b2) in
-      aux b1' b2';
-      let (Some (_, len1')) = parse (parse_list_bare p) b1' in
-      let (Some (_, len2')) = parse (parse_list_bare p) b2' in
-      Seq.lemma_split (Seq.slice b1 0 (len1 + len1')) len1;
-      Seq.lemma_split (Seq.slice b2 0 (len2 + len2')) len2;
-      assert (injective_postcond (parse_list_bare p) b1 b2)
-    end
-  in
-  Classical.forall_intro_2 (fun b -> Classical.move_requires (aux b))
-
-#reset-options
-
-inline_for_extraction
-let parse_list_kind =
-  {
-    parser_kind_low = 0;
-    parser_kind_high = None;
-    parser_kind_metadata = None;
-    parser_kind_subkind = Some ParserConsumesAll;
-  }
-
-abstract
-val parse_list
-  (#k: parser_kind)
-  (#t: Type0)
-  (p: parser k t)
-: Tot (parser parse_list_kind (list t))
-
 let parse_list #k #t p =
   parse_list_bare_injective p;
   parse_list_bare_consumes_all p;
   parser_kind_prop_equiv parse_list_kind (parse_list_bare p);
   parse_list_bare p
 
-abstract
 let parse_list_eq
   (#k: parser_kind)
   (#t: Type0)
@@ -158,7 +37,6 @@ let parse_list_eq
   ))
 = ()
 
-abstract
 let parse_list_eq'
   (#k: parser_kind)
   (#t: Type0)
@@ -180,24 +58,6 @@ let parse_list_eq'
         end
   )))
 = ()
-
-let rec bare_serialize_list
-  (#k: parser_kind)
-  (#t: Type0)
-  (p: parser k t)
-  (s: serializer p)
-  (x: list t)
-: GTot bytes
-= match x with
-  | [] -> Seq.empty
-  | a :: q -> Seq.append (s a) (bare_serialize_list p s q)
-
-unfold
-let serialize_list_precond
-  (k: parser_kind)
-: Tot bool
-= k.parser_kind_subkind = Some ParserStrong &&
-  k.parser_kind_low > 0
 
 let bare_serialize_list_correct
   (#k: parser_kind)
@@ -235,7 +95,6 @@ let bare_serialize_list_correct
   in
   Classical.forall_intro prf
 
-abstract
 let serialize_list
   (#k: parser_kind)
   (#t: Type0)
@@ -249,7 +108,6 @@ let serialize_list
 = bare_serialize_list_correct p s;
   bare_serialize_list p s
 
-abstract
 let serialize_list_nil
   (#k: parser_kind)
   (#t: Type0)
@@ -262,7 +120,6 @@ let serialize_list_nil
   (ensures (serialize (serialize_list p s) [] == Seq.empty))
 = ()
 
-abstract
 let serialize_list_cons
   (#k: parser_kind)
   (#t: Type0)
@@ -279,7 +136,6 @@ let serialize_list_cons
   ))
 = ()
 
-abstract
 let serialize_list_singleton
   (#k: parser_kind)
   (#t: Type0)
@@ -291,7 +147,6 @@ let serialize_list_singleton
   (ensures (serialize (serialize_list p s) [a] == serialize s a))
 = Seq.append_empty_r (serialize s a)
 
-abstract
 let rec serialize_list_append
   (#k: parser_kind)
   (#t: Type0)
@@ -308,210 +163,9 @@ let rec serialize_list_append
   | [] ->
     Seq.append_empty_l (serialize (serialize_list p s) l2)
 
-let rec serialize_list_eq_parser_fail
-  (#k: parser_kind)
-  (#t: Type)
-  (#p: parser k t)
-  (s: serializer p { k.parser_kind_subkind == Some ParserStrong /\ k.parser_kind_low > 0 })
-  (l1 l2: list t)
-  (b1 b2: bytes)
-: Lemma
-  (requires (
-    serialize (serialize_list _ s) l1 `Seq.append` b1 == serialize (serialize_list _ s) l2 `Seq.append` b2 /\
-    parse p b1 == None /\
-    parse p b2 == None
-  ))
-  (ensures (l1 == l2 /\ b1 == b2))
-  (decreases (L.length l1))
-= serialize_list_nil _ s;
-  assert (b1 `Seq.equal` (Seq.append Seq.empty b1));
-  assert (b2 `Seq.equal` (Seq.append Seq.empty b2));
-  if L.length l2 < L.length l1
-  then serialize_list_eq_parser_fail s l2 l1 b2 b1
-  else match l1, l2 with
-  | [], [] -> ()
-  | x1 :: l1', x2 :: l2' ->
-    serialize_list_cons _ s x1 l1' ;
-    serialize_list_cons _ s x2 l2' ;
-    Seq.append_assoc (serialize s x1) (serialize (serialize_list _ s) l1') b1;
-    Seq.append_assoc (serialize s x2) (serialize (serialize_list _ s) l2') b2;
-    serialize_strong_prefix s x1 x2 (serialize (serialize_list _ s) l1' `Seq.append` b1) (serialize (serialize_list _ s) l2' `Seq.append` b2);
-    serialize_list_eq_parser_fail s l1' l2' b1 b2
-  | [], x2 :: l2' ->
-    serialize_list_cons _ s x2 l2' ;
-    parse_strong_prefix p (serialize s x2) b1
-
-abstract
-let serialize_list_cons_upd
-  (#k: parser_kind)
-  (#t: Type0)
-  (#p: parser k t)
-  (s: serializer p)
-  (x: t)
-  (l2: list t)
-  (y: t)
-: Lemma
-  (requires (
-    serialize_list_precond k /\
-    Seq.length (serialize s y) == Seq.length (serialize s x)
-  ))
-  (ensures (
-    let ln2 = Seq.length (serialize (serialize_list _ s) l2) in
-    let sx = serialize s x in
-    let sl = serialize (serialize_list _ s) (x :: l2) in
-    Seq.length sl == Seq.length sx + ln2 /\
-    serialize (serialize_list _ s) (y :: l2) == seq_upd_seq sl 0 (serialize s y)
-  ))
-= serialize_list_cons _ s x l2;
-  serialize_list_cons _ s y l2;
-  let sl = serialize (serialize_list _ s) (x :: l2) in
-  seq_upd_seq_left sl (serialize s y);
-  let ln = Seq.length (serialize s x) in
-  Seq.lemma_split sl ln;
-  Seq.lemma_append_inj (Seq.slice sl 0 ln) (Seq.slice sl ln (Seq.length sl)) (serialize s x) (serialize (serialize_list _ s) l2)
-
-#set-options "--z3rlimit 32"
-
-abstract
-let serialize_list_upd
-  (#k: parser_kind)
-  (#t: Type0)
-  (#p: parser k t)
-  (s: serializer p)
-  (l1: list t)
-  (x: t)
-  (l2: list t)
-  (y: t)
-: Lemma
-  (requires (
-    serialize_list_precond k /\
-    Seq.length (serialize s y) == Seq.length (serialize s x)
-  ))
-  (ensures (
-    let ln1 = Seq.length (serialize (serialize_list _ s) l1) in
-    let ln2 = Seq.length (serialize (serialize_list _ s) l2) in
-    let sx = serialize s x in
-    let sl = serialize (serialize_list _ s) (l1 `L.append` (x :: l2)) in
-    Seq.length sl == ln1 + Seq.length sx + ln2 /\
-    serialize (serialize_list _ s) (l1 `L.append` (y :: l2)) == seq_upd_seq sl ln1 (serialize s y)
-  ))
-  (decreases (L.length l1))
-= serialize_list_append _ s l1 (y :: l2);
-  assert (serialize (serialize_list _ s) (l1 `L.append` (y :: l2)) == serialize (serialize_list _ s) l1 `Seq.append` serialize (serialize_list _ s) (y :: l2));
-  serialize_list_cons_upd s x l2 y;
-  assert (serialize (serialize_list _ s) (l1 `L.append` (y :: l2)) == serialize (serialize_list _ s) l1 `Seq.append` seq_upd_seq (serialize (serialize_list _ s) (x :: l2)) 0 (serialize s y));
-  seq_append_seq_upd_seq_l (serialize (serialize_list _ s) (x :: l2)) 0 (serialize s y) (serialize (serialize_list _ s) l1);
-  assert (serialize (serialize_list _ s) (l1 `L.append` (y :: l2)) == seq_upd_seq (serialize (serialize_list _ s) l1 `Seq.append` serialize (serialize_list _ s) (x :: l2)) (Seq.length (serialize (serialize_list _ s) l1) + 0) (serialize s y));
-  serialize_list_append _ s l1 (x :: l2)
-
-abstract
-let serialize_list_upd_bw
-  (#k: parser_kind)
-  (#t: Type0)
-  (#p: parser k t)
-  (s: serializer p)
-  (l1: list t)
-  (x: t)
-  (l2: list t)
-  (y: t)
-: Lemma
-  (requires (
-    serialize_list_precond k /\
-    Seq.length (serialize s y) == Seq.length (serialize s x)
-  ))
-  (ensures (
-    let ln1 = Seq.length (serialize (serialize_list _ s) l1) in
-    let ln2 = Seq.length (serialize (serialize_list _ s) l2) in
-    let sx = serialize s x in
-    let sl = serialize (serialize_list _ s) (l1 `L.append` (x :: l2)) in
-    Seq.length sl == ln1 + Seq.length sx + ln2 /\
-    serialize (serialize_list _ s) (l1 `L.append` (y :: l2)) == seq_upd_bw_seq sl ln2 (serialize s y)
-  ))
-  (decreases (L.length l1))
-= serialize_list_upd s l1 x l2 y
 
 #set-options "--z3rlimit 64"
 
-abstract
-let serialize_list_upd_chain
-  (#k: parser_kind)
-  (#t: Type0)
-  (#p: parser k t)
-  (s: serializer p)
-  (l1: list t)
-  (x: t)
-  (l2: list t)
-  (y: t)
-  (i' : nat)
-  (s' : bytes)
-: Lemma
-  (requires (
-    let sx = serialize s x in
-    serialize_list_precond k /\
-    i' + Seq.length s' <= Seq.length sx /\
-    serialize s y == seq_upd_seq sx i' s'
-  ))
-  (ensures (
-    let ln1 = Seq.length (serialize (serialize_list _ s) l1) in
-    let ln2 = Seq.length (serialize (serialize_list _ s) l2) in
-    let sx = serialize s x in
-    let sl = serialize (serialize_list _ s) (l1 `L.append` (x :: l2)) in
-    Seq.length sl == ln1 + Seq.length sx + ln2 /\
-    ln1 + i' + Seq.length s' <= Seq.length sl /\
-    serialize (serialize_list _ s) (l1 `L.append` (y :: l2)) == seq_upd_seq sl (ln1 + i') s'
-  ))
-= serialize_list_upd s l1 x l2 y;
-  serialize_list_append _ s l1 (x :: l2);
-  let sl1 = serialize (serialize_list _ s) l1 in
-  let ln1 = Seq.length sl1 in
-  let sxl2 = serialize (serialize_list _ s) (x :: l2) in
-  let sl = serialize (serialize_list _ s) (l1 `L.append` (x :: l2)) in
-  Seq.lemma_split sl ln1;
-  Seq.lemma_append_inj (Seq.slice sl 0 ln1) (Seq.slice sl ln1 (Seq.length sl)) sl1 sxl2;
-  let sx = serialize s x in
-  let sl2 = serialize (serialize_list _ s) l2 in
-  let lx = Seq.length sx in
-  serialize_list_cons _ s x l2;
-  Seq.lemma_split sxl2 lx;
-  Seq.lemma_append_inj (Seq.slice sxl2 0 lx) (Seq.slice sxl2 lx (Seq.length sxl2)) sx sl2;
-  Seq.slice_slice sl ln1 (Seq.length sl) 0 lx;
-  assert (sx == Seq.slice sl ln1 (ln1 + lx));
-  seq_upd_seq_seq_upd_seq_slice sl ln1 (ln1 + lx) i' s';
-  ()
-
-abstract
-let serialize_list_upd_bw_chain
-  (#k: parser_kind)
-  (#t: Type0)
-  (#p: parser k t)
-  (s: serializer p)
-  (l1: list t)
-  (x: t)
-  (l2: list t)
-  (y: t)
-  (i' : nat)
-  (s' : bytes)
-: Lemma
-  (requires (
-    let sx = serialize s x in
-    serialize_list_precond k /\
-    i' + Seq.length s' <= Seq.length sx /\
-    serialize s y == seq_upd_bw_seq sx i' s'
-  ))
-  (ensures (
-    let ln1 = Seq.length (serialize (serialize_list _ s) l1) in
-    let ln2 = Seq.length (serialize (serialize_list _ s) l2) in
-    let sx = serialize s x in
-    let sl = serialize (serialize_list _ s) (l1 `L.append` (x :: l2)) in
-    Seq.length sl == ln1 + Seq.length sx + ln2 /\
-    ln2 + i' + Seq.length s' <= Seq.length sl /\
-    serialize (serialize_list _ s) (l1 `L.append` (y :: l2)) == seq_upd_bw_seq sl (ln2 + i') s'
-  ))
-= let sx = serialize s x in
-  let j' = Seq.length sx - i' - Seq.length s' in
-  serialize_list_upd_chain s l1 x l2 y j' s'
-
-abstract
 let serialize_list_cons_upd_chain
   (#k: parser_kind)
   (#t: Type0)
@@ -539,36 +193,6 @@ let serialize_list_cons_upd_chain
   ))
 = serialize_list_upd_chain s [] x l2 y i' s'
 
-abstract
-let serialize_list_cons_upd_bw_chain
-  (#k: parser_kind)
-  (#t: Type0)
-  (#p: parser k t)
-  (s: serializer p)
-  (x: t)
-  (l2: list t)
-  (y: t)
-  (i' : nat)
-  (s' : bytes)
-: Lemma
-  (requires (
-    let sx = serialize s x in
-    serialize_list_precond k /\
-    i' + Seq.length s' <= Seq.length sx /\
-    serialize s y == seq_upd_bw_seq sx i' s'
-  ))
-  (ensures (
-    let ln2 = Seq.length (serialize (serialize_list _ s) l2) in
-    let sx = serialize s x in
-    let sl = serialize (serialize_list _ s) (x :: l2) in
-    Seq.length sl == Seq.length sx + ln2 /\
-    ln2 + i' + Seq.length s' <= Seq.length sl /\
-    serialize (serialize_list _ s) (y :: l2) == seq_upd_bw_seq sl (ln2 + i') s'
-  ))
-= let j' = Seq.length (serialize s x) - i' - Seq.length s' in
-  serialize_list_cons_upd_chain s x l2 y j' s'
-
-abstract
 let serialize_list_snoc_upd_chain
   (#k: parser_kind)
   (#t: Type0)
@@ -596,55 +220,8 @@ let serialize_list_snoc_upd_chain
   ))
 = serialize_list_upd_chain s l1 x [] y i' s'
 
-abstract
-let serialize_list_snoc_upd_bw_chain
-  (#k: parser_kind)
-  (#t: Type0)
-  (#p: parser k t)
-  (s: serializer p)
-  (l1: list t)
-  (x: t)
-  (y: t)
-  (i' : nat)
-  (s' : bytes)
-: Lemma
-  (requires (
-    let sx = serialize s x in
-    serialize_list_precond k /\
-    i' + Seq.length s' <= Seq.length sx /\
-    serialize s y == seq_upd_bw_seq sx i' s'
-  ))
-  (ensures (
-    let ln1 = Seq.length (serialize (serialize_list _ s) l1) in
-    let sx = serialize s x in
-    let sl = serialize (serialize_list _ s) (l1 `L.append` [x]) in
-    Seq.length sl == ln1 + Seq.length sx /\
-    i' + Seq.length s' <= Seq.length sl /\
-    serialize (serialize_list _ s) (l1 `L.append` [y]) == seq_upd_bw_seq sl i' s'
-  ))
-= let j' = Seq.length (serialize s x) - i' - Seq.length s' in
-  serialize_list_snoc_upd_chain s l1 x y j' s'
 
 #reset-options
-
-abstract
-val list_length_constant_size_parser_correct
-  (#k: parser_kind)
-  (#t: Type0)
-  (p: parser k t)
-  (b: bytes)
-: Lemma
-  (requires (
-    k.parser_kind_high == Some k.parser_kind_low /\
-    Some? (parse (parse_list p) b)
-  ))
-  (ensures (
-    let pb = parse (parse_list p) b in
-    Some? pb /\ (
-    let (Some (l, _)) = pb in
-    FStar.Mul.op_Star (L.length l) k.parser_kind_low == Seq.length b
-  )))
-  (decreases (Seq.length b))
 
 let rec list_length_constant_size_parser_correct #k #t p b =
   parser_kind_prop_equiv k p;
@@ -659,34 +236,4 @@ let rec list_length_constant_size_parser_correct #k #t p b =
     list_length_constant_size_parser_correct p b';
     let (Some (l', _)) = parse (parse_list p) b' in
     FStar.Math.Lemmas.distributivity_add_left 1 (L.length l') n
-  end
-
-abstract
-let rec parse_list_total_constant_size
-  (#k: parser_kind)
-  (#t: Type0)
-  (p: parser k t)
-  (elem_count: nat)
-  (x: bytes)
-: Lemma
-  (requires (
-    serialize_list_precond k /\
-    k.parser_kind_high == Some k.parser_kind_low /\
-    k.parser_kind_metadata == Some ParserKindMetadataTotal /\
-    Seq.length x == elem_count `Prims.op_Multiply` k.parser_kind_low
-  ))
-  (ensures (
-    Some? (parse (parse_list p) x)
-  ))
-  (decreases elem_count)
-= parse_list_eq p x;
-  if elem_count = 0
-  then ()
-  else begin
-    assert (Seq.length x == k.parser_kind_low + ((elem_count - 1) `Prims.op_Multiply` k.parser_kind_low));
-    parser_kind_prop_equiv k p;
-    assert (Some? (parse p x));
-    let Some (_, len) = parse p x in
-    assert (len == k.parser_kind_low);
-    parse_list_total_constant_size p (elem_count - 1) (Seq.slice x len (Seq.length x))
   end
